Provbide a module to parse commandline arguments. Fixes #8

src/dafny/utils/parseArgs.dfy
@@ -12,66 +12,207 @@
  * under the License.
  */
 
-/** Provide parsing of commadline optios. */
-module parseArgs {
+include "./MiscTypes.dfy"
+include "./int.dfy"
 
+/** Provide parsing of commadline options. 
+  * 
+  * Usage: see at the end of the module for an example method.
+  */
+module ArgParser {
+
+  import opened MiscTypes
+  import Int
+
+  datatype CLIOption = CLIOption(name: string, numArgs: nat, desc: string)
   class Args {
 
+
     /** The list of known options.
-      * Argument name, and number of expected arguments for the option.
+      * Argument name, and number of expected arguments/help for the option.
       */
-    var knownArgs: map<string, nat>
+    var knownArgs: map<string, CLIOption>
+    var knownNameArgs: map<string, string>
 
     /** The list of known keys. Useful to iterate over keys in a map. */
     var knownKeys: seq<string>
 
     /**
-     *  Ensure the list of keys is the same as the list of knownArgs keys.
-     */
+      *  Ensure the list of keys is the same as the list of knownArgs keys.
+      */
     ghost predicate Inv()
       reads this
     {
-      multiset(knownArgs.Keys) == multiset(knownKeys)
+      && multiset(knownArgs.Keys) == multiset(knownKeys)
+      && knownNameArgs.Values <= knownArgs.Keys
     }
 
+    /**
+      * Initialise the args.
+      */
     constructor()
       ensures Inv()
     {
-      knownArgs := map[];
-      knownKeys := [];
+      knownArgs := map["-h" := CLIOption("--help", 0, "Display help and exit")];
+      knownNameArgs := map["--help" := "-h"];
+      knownKeys := ["-h"];
     }
 
-    method {:verify true} AddOption(name: string, numArgs: nat := 0, help: string := "No help")
+    /**
+      * Register a new option.
+      * 
+      * @param  opname  The short name of the option, e.g. "-h" or "-a"
+      * @param  name    The longname of the option, e.g. "--help" or "--file"
+      * @param  numArgs The number of arguments that the option takes. E.g. if "--file" should
+      *                 be followed by one argument, it is 1. Default value is 0.
+      * @param  help    The description of the option.
+      *
+      * @note   If the option name already exists, it is overriden.
+      */
+    method {:verify true} AddOption(opname: string, name: string, numArgs: nat := 0, help: string := "No help provided")
       requires Inv()
-      modifies `knownArgs, `knownKeys
+      modifies `knownArgs, `knownKeys, `knownNameArgs
       ensures Inv()
     {
-      knownArgs := knownArgs[name := numArgs];
-      if name !in knownKeys {
-        knownKeys := knownKeys + [name];
+      knownArgs := knownArgs[opname := CLIOption(name, numArgs, help)];
+      knownNameArgs := knownNameArgs[name := opname];
+      if opname !in knownKeys {
+        knownKeys := knownKeys + [opname];
       }
-
     }
 
-    method {:verify true} Print()
+    /**
+      *  Print out the help of options and the number of arguments and help.
+      */
+    method {:verify true} PrintHelp()
       requires Inv()
       ensures Inv()
     {
+      print "usage: <this program> ";
       for i := 0 to |knownKeys| {
         assert knownKeys[i] in multiset(knownKeys);
-        print knownKeys[i], " ", knownArgs[knownKeys[i]];
+        var k := knownArgs[knownKeys[i]];
+        print " [", knownKeys[i], "] ";
+        //  print arguments
+        for i := 0 to k.numArgs {
+          print  " arg", i;
+        }
       }
+      print "\n\n";
+      //    Display option help one per line
+      print "options", "\n";
+      var maxL := MaxValueFast(knownKeys);
+
+      for i := 0 to |knownKeys| {
+        assert knownKeys[i] in multiset(knownKeys);
+        var k := knownArgs[knownKeys[i]];
+        SameMax(knownKeys);
+        print knownKeys[i], seq(maxL - |knownKeys[i]| + 2, _ => ' ') , " [", k.name, "] ", k.desc ; // , " ", k.0;
+        print "\n";
+      }
+    }
+
+    /**
+      * Parse the commandline arguments and collect options' values.
+      *
+      * @param  args            The arguments to be parsed.
+      * @param  alreadyParsed   The already collected option values.
+      * @returns                A Success with a map, mapping option long names with their
+      *                         list of arguments or Failure is parsing fails.
+      *                         If it succeeds, the map contains the entries that correspond
+      *                         to options in the command line arguments.
+      *                         The key to the option is the long name, e.g. for am option "-f" with
+      *                         longname "--file", the entry for "-f" or "--file" will be at "--file".
+      * @example                if "--file" is declared with 1 argument, parsing "--file" filename
+      *                         succeeds. If ""-file" is not followed by one argument, it fails.
+      * @example                Note that "--file" "--quiet" will succeed and interpret "--quiet" as 
+      *                         the argument of "--file".
+      */
+    function ParseArgs(args: seq<string>, alreadyParsed: map<string, seq<string>> := map[]): Try<map<string, seq<string>>>
+      reads this
+      requires Inv()
+      ensures Inv()
+    {
+      //  parse the seq and retrieve the values of known options.
+      if |args| == 0 then Success(alreadyParsed)
+      else
+      if args[0] in knownArgs.Keys || args[0] in knownNameArgs.Keys then
+        //  read the number of arguments if possible, and otherwise
+        //  fail.
+        // Retrieve option
+        var opt := if args[0] in knownArgs.Keys then knownArgs[args[0]]
+                   else knownArgs[knownNameArgs[args[0]]];
+        var numArgs := opt.numArgs;
+        if |args[1..]| < numArgs then
+          Failure("argument " + args[0] + " needs more arguments")
+        else
+          //   read them
+          var r := args[1..][..numArgs];
+          ParseArgs(args[1 + numArgs..], alreadyParsed[opt.name := r])
+
+      else ParseArgs(args[1..], alreadyParsed)
+    }
+
+    //  Helper
+
+    /**
+      *  Max length of elements in the sequence.
+      */
+    ghost function MaxValue(s: seq<string>): (r: nat)
+      ensures forall i:: 0 <= i < |s| ==> |s[i]| <= r
+    {
+      if |s| == 0 then 0
+      else Int.Max(|s[0]|, MaxValue(s[1..]))
+    }
+
+    /**
+      * Tail recursive computation of max value.
+      */
+    function {:tailrecursion true} MaxValueFast(s: seq<string>, max: nat := 0): (r: nat)
+    {
+      if |s| == 0 then max
+      else MaxValueFast(s[1..], Int.Max(|s[0]|, max))
+    }
+
+    //  Some useful lemmas
+
+    lemma SameMax(s: seq<string>)
+      ensures MaxValue(s) == MaxValueFast(s, 0)
+      ensures forall i:: 0 <= i < |s| ==> |s[i]| <= MaxValueFast(s)
+    {
+      if |s| > 0 {
+        SameMaxExtractFirst(s[1..], s[0]);
+      }
+    }
+
+    lemma SameMaxExtractFirst(s: seq<string>, e: string)
+      ensures MaxValue([e] + s) == MaxValueFast(s, |e|)
+    {
+      //  Thanks Dafny
     }
   }
 
-  method {:main} Main() {
-    print "hello\n";
+  method {:test} Main() {
+    print "hello! Testing parseArg!\n";
     var cli := new Args();
-    cli.AddOption("-one");
+    cli.AddOption("-o", "--one");
+    cli.AddOption("-tw", "--two", 2, "don't do that!");
 
-    cli.Print();
-    print "\n";
-    print cli.knownKeys, "\n";
+    var r := cli.ParseArgs(["-one", "--two", "a1", "a2", "-unknwon"]);
+
+    match r {
+      case Success(m) =>
+        if "-o" in m.Keys {
+          print "Success -o!", m["-o"], "\n" ;
+        }
+        if "--two" in m.Keys {
+          print "Success -two!", m["--two"], "\n" ;
+        }
+      case Failure(msg) =>
+        print msg, "\n";
+
+    }
+    cli.PrintHelp();
 
   }
 
